example WIP.

theories/examples/run_yield_1.v
@@ -3,7 +3,8 @@ From HypVeri Require Import reg_addr RAs rule_misc lifting.
 From HypVeri.rules Require Import rules_base mov ldr str halt run yield.
 From iris.proofmode Require Import tactics.
 From iris.base_logic.lib Require Export invariants.
-Require Import iris.base_logic.lib.ghost_map iris.bi.big_op iris.algebra.lib.frac_agree.
+From iris.algebra Require Import excl.
+(* iris.base_logic.lib.ghost_map iris.bi.big_op *)
 Require Import stdpp.fin.
 
 Section RunYield1.
@@ -31,61 +32,84 @@ Section RunYield1.
     hvc_I
     ].
   
-  Class tokG Σ := tok_G :> inG Σ (frac_agreeR (leibnizO vmid)).
+  Class tokG Σ := tok_G :> inG Σ (exclR unitO).
 
   Context `{gen_VMG Σ, tokG Σ}.
 
   Definition program (instr: list Word) (b:Addr):=
     ([∗ list] a;w ∈ (finz.seq b (length instr));instr, (a ->a w))%I.
 
-  Definition tokI γ i := own γ (to_frac_agree (1/2)%Qp i).
-  
-  Definition tokN := nroot .@ "tok".
+  Definition tokI γ := own γ (Excl ()).
 
-  Definition is_tok γ (z i:VMID) :=
-    inv tokN ((<<z>>) ∨ ∃j, tokI γ j ∗ ⌜j = i⌝ ∗ <<i>>)%I.
+  Lemma tokI_excl γ : tokI γ -∗ tokI γ -∗ False.
+  Proof.
+    iIntros "H1 H2".
+    unfold tokI.
+    iDestruct (own_valid_2 with "H1 H2") as "%HF".
+    iPureIntro.
+    inversion HF.
+    Qed.
 
-  (* Definition seq_in_a_page (b e: Addr) (p:PID) := *)
-  (*   ((of_pid p) <=? b)%f ∧ (e <? ((of_pid p) ^+ page_size))%f. *)
+  Definition invN := nroot .@ "tok".
 
-  Lemma spec1 {γ z i q1 q2 prog1page prog2page r0_} :
+  Definition inv γ1 γ2 (z i:VMID) :=
+    inv invN ((<<z>>) ∗ tokI γ1 ∨   <<i>> ∗ tokI γ2)%I.
+  (* it seems we may need a more complicated invariant... *)
+
+
+  Lemma mach_zero {γ1 γ2 z i q1 prog1page r0_} :
+      fin_to_nat z = 0 ->
+      z ≠ i ->
+      program (program1 i) (of_pid prog1page) ∗
+      ⌜ seq_in_a_page (of_pid prog1page) (length (program1 i)) prog1page ⌝ ∗
+      inv γ1 γ2 z i ∗  tokI γ2 ∗
+      A@z :={q1} prog1page
+      ∗ PC @@ z ->r (of_pid prog1page)
+      ∗ R0 @@ z ->r r0_
+      ⊢ (WP ExecI @ z {{ (λ m, ⌜m = HaltI⌝) }}%I).
+  Proof.
+    iIntros (zP neH) "((p_1 & p_2 & p_3 & p_4 & _) & %Hinpage & #Hinv & Hgtok2 & Hacc & PCz & R0z)".
+    rewrite wp_sswp.
+    iApply (sswp_fupd_around ⊤ ⊤ ⊤).
+    iInv invN as ">S" "HClose".
+    iDestruct "S" as "[[Htok Hgtok] | [Htok Hgtok] ]".
+    - iDestruct
+      ((@mov_word _ _ (Mov R0 (inl run_I)) z (mov_word_I R0 run_I) r0_ q1 (of_pid prog1page) run_I R0)
+         with "[Htok p_1 PCz Hacc R0z]") as "J"; eauto.
+      * by rewrite decode_encode_instruction.
+      * iFrame.
+      * admit.
+    - iDestruct "S" as "(Hgtok & Htok)".
+      iExFalso.
+      iApply (tokI_excl with "Hgtok2 Hgtok").
+  Qed.
+
+
+  Lemma spec1 {γ1 γ2 z i q1 q2 prog1page prog2page r0_} :
       fin_to_nat z = 0 ->
       z ≠ i ->
       program (program1 i) (of_pid prog1page) ∗
       program (program2) (of_pid prog2page) ∗
-      is_tok γ z i ∗
+      inv γ1 γ2 z i ∗ tokI γ1 ∗ tokI γ2 ∗
       A@z :={q1} prog1page ∗ A@i :={q2} prog2page
       ∗ PC @@ z ->r (of_pid prog1page) ∗ PC @@ i ->r (of_pid prog2page)
       ∗ R0 @@ z ->r r0_
       ⊢ (WP ExecI @ z {{ (λ m, ⌜m = HaltI⌝) }}%I)
        ∗ (WP ExecI @ i {{ (λ m, ⌜m = ExecI⌝) }}%I).
   Proof.
-    iIntros (zP neH) "((p_1 & p_2 & p_3 & p_4 & _) & (p_1' & p_2' & _) & #Hinv & Hacc1 & Hacc2 & PCz & PCi & Hr0_)".
-    iSplitL "p_1 p_2 p_3 p_4 Hacc1 PCz Hr0_".
+    iIntros (zP neH) "((p_1 & p_2 & p_3 & p_4 & _) & (p_1' & p_2' & _) & #Hinv & Hgtok1 & Hgtok2 & Hacc1 & Hacc2 & PCz & PCi & Hr0_)".
+    iSplitL "p_1 p_2 p_3 p_4 Hgtok2 Hacc1 PCz Hr0_".
     - rewrite wp_sswp.
       iApply (sswp_fupd_around ⊤ ⊤ ⊤).
-      iInv tokN as ">S" "HClose".
+      iInv invN as ">S" "HClose".
       iDestruct "S" as "[S | S]".
       + iDestruct ((@mov_word _ _ (Mov R0 (inl run_I)) z (mov_word_I R0 run_I) r0_ q1 (of_pid prog1page) run_I R0) with "[> S]") as "J"; eauto.
         * by rewrite decode_encode_instruction.          
         * admit.
         * admit.
-      + iDestruct "S" as "[%j (S1 & %S2 & S3)]".
-        simplify_eq.
-        iApply (sswp_mono z _ ExecI (λ _, False %I) _).
-        * iIntros;iExFalso; done.
-        * assert (neH' : i ≠ z).
-          {
-            intros contra.
-            apply neH.
-            symmetry.
-            assumption.
-          }
-          iApply eliminate_wrong_token.
-          (* TODO eliminate_wrong_token consumes the token, so we cannot close the invariant! *)
-          apply neH'.
-          iFrame.
-          admit.
+      + iDestruct "S" as "(Hgtok & Htok)".
+        iExFalso.
+        iApply (tokI_excl with "Hgtok2 Hgtok").
     - admit.
 Admitted.
 
