theories/reg_addr.v
@@ -1,4 +1,4 @@
-From Coq Require Import ssreflect ZArith.
+From Coq Require Import ssreflect Eqdep_dec ZArith.
 From HypVeri Require Import machine monad.
 From stdpp Require Import fin_maps list countable fin vector.
 
@@ -29,3 +29,125 @@ Solve Obligations with solveRegCount.
 
 Program Definition R2 :reg_name := (R 2 _).
 Solve Obligations with solveRegCount.
+
+
+  (** predicates and lemmas for checking if addresses/regions are in a page *)
+  Definition addr_in_page (a: Addr ) (p:PID):=
+    ((of_pid p) <=? a)%f ∧ (a <=? ((of_pid p) ^+ (page_size -1 )))%f.
+
+  Definition seq_in_page (b :Addr) (l: nat) (p:PID) :=
+    ((of_pid p) <=? b)%Z ∧ is_Some (b + (Z.of_nat l))%f ∧ ((b ^+ (Z.of_nat l))%f <=? ((of_pid p) ^+ (page_size-1))%f)%Z.
+
+  Lemma last_addr_in_bound (p:PID):
+    is_Some ((of_pid p) + (page_size -1)%Z)%f.
+    Proof.
+      destruct p.
+      destruct z.
+      simplify_eq /=.
+      assert (Hy : exists y, (y * page_size = word_size)%Z).
+      exists 2000%Z.
+      unfold page_size, word_size.
+      lia.
+      destruct Hy.
+      assert (Hlt: (z + page_size -1 < word_size)%Z).
+      {
+       apply Z.ltb_lt in finz_lt.
+       apply Z.leb_le in finz_nonneg.
+       assert (Hlt': (z  < word_size - page_size + 1 )%Z).
+       {
+         destruct (decide (z  < word_size - page_size + 1)%Z).
+         lia.
+         assert(H': ( (x -1 ) * page_size < z )%Z).
+         lia.
+         apply Z.rem_divide in align;[|unfold page_size;lia].
+         destruct align.
+         subst z.
+         rewrite -H in finz_lt.
+         apply Zmult_gt_0_lt_reg_r in finz_lt;[|unfold page_size;lia].
+         apply Zmult_gt_0_lt_reg_r in H';[|unfold page_size;lia].
+         lia.
+       }
+       lia.
+       }
+      unfold finz.incr.
+      simpl.
+      destruct (Z_lt_dec (z + (page_size - 1))%Z word_size).
+      destruct (Z_le_dec 0%Z (z + (page_size - 1))%Z).
+      eauto.
+      exfalso.
+      apply n.
+      unfold page_size.
+      lia.
+      exfalso.
+      apply n.
+      lia.
+  Qed.
+
+    Lemma last_addr_in_bound' p f : ((of_pid p) + (page_size -1)%Z)%f = Some f ->
+                                    ((of_pid p) ^+ (page_size -1)%Z)%f = f.
+      Proof.
+        intro.
+        unfold finz.incr_default.
+        by rewrite H.
+      Qed.
+
+
+  Lemma to_pid_aligned_in_page (a:Addr) (p:PID) :
+    addr_in_page a p -> (to_pid_aligned a ) = p.
+    Proof.
+      intro.
+      unfold to_pid_aligned.
+      unfold addr_in_page in H.
+      destruct H.
+      pose proof (last_addr_in_bound p).
+      destruct H1.
+      rewrite (last_addr_in_bound' p x) in H0;eauto.
+      destruct p.
+      destruct z.
+      f_equal /=.
+      assert (Heq : z = (page_size * (a / page_size))%Z).
+      {
+        destruct a.
+        simplify_eq /=.
+        destruct (decide (z = z0 )%Z);eauto.
+        rewrite -e.
+         apply Z.rem_mod_eq_0 in align.
+          apply Z_div_exact_2.
+          unfold page_size;lia.
+          lia.
+          unfold page_size;lia.
+
+        unfold finz.leb in H.
+        simpl in H.
+        unfold finz.ltb in H0.
+        simpl in H0.
+        apply Is_true_eq_true in H, H0.
+        apply Z.leb_le in H.
+        assert (Heq : (z < z0)%Z).
+        {
+          lia.
+        }
+        apply Z.leb_le in H0.
+        simpl in H0 ,H1 .
+        apply Z.rem_divide in align;[|unfold page_size;lia].
+        admit.
+      }
+      subst z.
+      remember (machine.to_pid_aligned_obligation_3 a) as Ha'.
+      simpl in Ha'.
+      assert (Heqiv : Ha' = align).
+      apply eq_proofs_unicity; decide equality; decide equality.
+      rewrite Heqiv.
+      repeat f_equal /=.
+      remember (machine.to_pid_aligned_obligation_1 a) as Ha''.
+      simpl in  Ha''.
+      remember (machine.to_pid_aligned_obligation_2 a) as Ha'''.
+      simpl in  Ha'''.
+      assert (Heqiv' : Ha'' = finz_lt).
+      apply eq_proofs_unicity; decide equality; decide equality.
+      rewrite Heqiv'.
+      assert (Heqiv'' : Ha''' = finz_nonneg).
+      apply eq_proofs_unicity; decide equality; decide equality.
+      rewrite Heqiv''.
+      done.
+Qed.
